proofs/FEC/ProducerConsumerCorrectness.v
@@ -1,5 +1,5 @@
-Require Import Encoder.
-Require Import DecoderMachine.
+Require Import Producer.
+Require Import ConsumerMachine.
 From mathcomp Require Import all_ssreflect.
 Set Implicit Arguments.
 Unset Strict Implicit.
@@ -26,42 +26,42 @@ Theorem all_decoded_in_Z: forall (orig : list packet) (encoded received: list fp
   (forall p, p \in orig -> packet_valid p) ->
   (forall p, p \in orig -> encodable p) ->
   uniq (map p_seqNum orig) ->
-  encoded = (encoder_all_steps orig enc_params).2 ->
+  encoded = (producer_all_steps orig enc_params).2 ->
   (forall p, p \in received -> p \in encoded) ->
-  decoded = (decoder_all_steps_gen upd_time not_timeout received).1.2 ->
+  decoded = (consumer_all_steps_gen upd_time not_timeout received).1.2 ->
   forall p, p \in decoded -> exists p', p' \in orig /\ remove_seqNum p = remove_seqNum p'.
 Proof.
   move => orig encoded received decoded enc_params Hleno Hencparams Hallvalid Hallenc Hseqnum
     Henc Hloss Hdec p Hind; subst.
-  (*Step 1: since p is in the decoder, it must have been in [rse_decode_func] at some point*)
-  move: Hind. rewrite decoder_all_steps_concat // in_mem_In in_concat => [[dec]] [Hinp].
+  (*Step 1: since p is in the Consumer, it must have been in [rse_consume_func] at some point*)
+  move: Hind. rewrite consumer_all_steps_concat // in_mem_In in_concat => [[dec]] [Hinp].
   rewrite In_Znth_iff; zlist_simpl => [[i] [Hi]]. zlist_simpl. move => Hdec. subst. move: Hinp. rewrite -in_mem_In => Hp.
   have Hleno': size orig = size enc_params by rewrite !size_Zlength Hleno.
-  have Hwfenc: wf_packet_stream (encoder_all_steps orig enc_params).2 by apply rse_encode_stream_wf.
+  have Hwfenc: wf_packet_stream (producer_all_steps orig enc_params).2 by apply rse_produce_stream_wf.
   have Hwfrec: wf_packet_stream received by apply (wf_substream Hwfenc).
   have Hidx: 0 <= Z.of_nat (fd_blockIndex (Znth i received)) < fd_k (Znth i received) + fd_h (Znth i received). {
     split; try lia; apply Hwfrec. rewrite in_mem_In. by apply Znth_In. }
   have Hcurrh: 0 <= fd_h (Znth i received). { apply Hwfrec. rewrite in_mem_In. by apply Znth_In. }
   have Hsubstream: forall x : fpacket_eqType,
     x \in Znth i received :: sublist 0 i received ->
-    x \in (encoder_all_steps orig enc_params).2. {
+    x \in (producer_all_steps orig enc_params).2. {
       move=> x. rewrite in_cons => /orP[/eqP Hx | Hinrec].
       - rewrite Hx. apply Hloss. apply /inP. by apply Znth_In.
       - apply Hloss. by apply (mem_sublist Hinrec).
     }
   (*Step 2: Thus, p either was in received or was produced by running [decode_block].*) 
-  apply in_decode_func_in_block in Hp =>//.
+  apply in_consume_func_in_block in Hp =>//.
   case : Hp => [[Hp Hpar] | [b1 [b2 [Hinb2 [Hsub [Hrec Hpin]]]]]].
-  - (*In the first case, this is easy, since all data packets produced by the encoder are in the original stream*)
-    exists p. split => //. rewrite -Hp. apply (rse_encode_stream_from_orig Hencparams) => //.
+  - (*In the first case, this is easy, since all data packets produced by the Producer are in the original stream*)
+    exists p. split => //. rewrite -Hp. apply (rse_produce_stream_from_orig Hencparams) => //.
     apply Hloss. rewrite in_mem_In. by apply Znth_In.
   - (*In the second case, we use lots of previous results. Namely, we need to know that b is a subblock of
       some block b' that is well-formed and encoded (it comes directly from the encoder). We need 2 layers, 
-      since the subblock in the decoder is a subblock of a block in (get_blocks received), which is a subblock
+      since the subblock in the Consumer is a subblock of a block in (get_blocks received), which is a subblock
       of a block from (get_blocks encoded). Once we have this, we can use [in_decode_block_in_data], which
       uses the correctness of the (Reed Solomon) decoder*)
     have [b' [Hsubb' [Hwfb' [Hencb' Hgetb]]]]: exists b', subblock b1 b' /\ block_wf b' /\ block_encoded b' /\
-      b' \in (get_blocks (encoder_all_steps orig enc_params).2) . {
+      b' \in (get_blocks (producer_all_steps orig enc_params).2) . {
       (*Idea: b2 is a subblock of something in received (by sublist), 
         which is a subblock of something in encoded (by sublist), then
         we use transitivity*)
@@ -69,15 +69,15 @@ Proof.
         (get_blocks_sublist Hwfenc Hsubstream Hinb2).
       exists b3. split_all=>//.
       - by apply (subblock_trans Hsub).
-      - by apply (rse_encode_stream_blocks_wf Hencparams Hallvalid).
-      - apply (rse_encode_stream_recoverable_encoded Hencparams Hallvalid) => //.
+      - by apply (rse_produce_stream_blocks_wf Hencparams Hallvalid).
+      - apply (rse_produce_stream_recoverable_encoded Hencparams Hallvalid) => //.
         by apply (subblock_recoverable (subblock_trans Hsub Hsubb3)).
     }
     (*Now we apply [in_decode_block_in_data]*)
     have [p' [Hpin' Hpnum]]:=in_decode_block_in_data Hwfb' Hencb' Hsubb' Hrec Hpin.
     exists (p_packet p'). split => //.
     have Hpar': fd_isParity p' = false. apply Hwfb'=>//. 
-    apply (rse_encode_stream_from_orig Hencparams) => //.
+    apply (rse_produce_stream_from_orig Hencparams) => //.
     apply (get_blocks_in_orig Hwfenc Hgetb). by apply data_in_block.
   - by apply (wf_substream Hwfenc Hsubstream).
 Qed.
@@ -119,7 +119,7 @@ Theorem block_i_recovered_Z (orig : list packet)
   uniq (map p_seqNum orig) ->
   Zlength enc_params = Zlength orig ->
   all (fun x => x == (k, h)) enc_params ->
-  encoded = (encoder_all_steps orig enc_params).2 ->
+  encoded = (producer_all_steps orig enc_params).2 ->
   (*No new packets are added*)
   (forall p, p \in received -> p \in encoded) ->
   (*At least k packets in i(k+h) to (i+1) (k+h) received*)
@@ -128,7 +128,7 @@ Theorem block_i_recovered_Z (orig : list packet)
   (*Bound on reordering and duplication*)
   duplicates_bounded received fpacket_inhab m ->
   reorder_bounded encoded received d ->
-  decoded = (decoder_all_steps threshold received).1.2 ->
+  decoded = (consumer_all_steps threshold received).1.2 ->
   (*Threshold is large enough*)
   (threshold >= k + h + Z.of_nat (2 * d + m))%Z ->
   (*Then any packet from ik to (i+1)k in the original list
@@ -139,26 +139,26 @@ Theorem block_i_recovered_Z (orig : list packet)
 Proof.
   move => Hallvalid Hallenc Hseqnum Hlenenc Hallkh Henc Hsub Hi Hloss Hdups 
     Hreord Hdec Hthresh p Hinp.
-  (*First, we use [encoder_concat_nochange_eq] to reason about
-    the encoder with no parameter changes*)
+  (*First, we use [producer_concat_nochange_eq] to reason about
+    the Producer with no parameter changes*)
   have Henceq: enc_params = zseq (Zlength orig) (k, h) by
     apply zseq_eq.
   rewrite Henceq in Henc. clear Hlenenc Hallkh Henceq enc_params.
-  move: Henc. rewrite encoder_all_steps_concat 
-    -encoder_concat_nochange_eq => Henc.
-  (*Next, use [encoder_boundaries_i] to get the boundary*)
-  have:=(encoder_boundaries_i k_bound h_bound 
+  move: Henc. rewrite producer_all_steps_concat 
+    -producer_concat_nochange_eq => Henc.
+  (*Next, use [producer_boundaries_i] to get the boundary*)
+  have:=(producer_boundaries_i k_bound h_bound 
     Hallvalid Hallenc Hseqnum Hinp Hi)=>/=.
   rewrite -Henc.
-  set (b := nth block_inhab (rev (encoder_concat_nochange k h orig).1.1) i).
+  set (b := nth block_inhab (rev (producer_concat_nochange k h orig).1.1) i).
   move=> [Hinb [Hencb [Hwfb [Hbk [Huniq [Hall [Hszenc [f [Hpf [Hparf Hinfb]]]]]]]]]].
-  (*Now, we use [decoder_timeout_notimeout_all] to show that the
-    decoder is equivalent to one without timeouts. We first need
+  (*Now, we use [consumer_timeout_notimeout_all] to show that the
+    Consumer is equivalent to one without timeouts. We first need
     the preconditions:*)
   have Hwf: wf_packet_stream encoded. {
     (*ugh, dont want to reverse*)
-    rewrite Henc encoder_concat_nochange_eq -encoder_all_steps_concat.
-    apply rse_encode_stream_wf=>//.
+    rewrite Henc producer_concat_nochange_eq -producer_all_steps_concat.
+    apply rse_produce_stream_wf=>//.
     - move=> k' h'. by rewrite /zseq mem_nseq => /andP[_ /eqP[]->->].
     - by rewrite /zseq size_nseq Zlength_size Nat2Z.id.
   } 
@@ -173,15 +173,15 @@ Proof.
         far apart *)
       move=> p1 p2 Hinp1 Hinp2 Hideq.
       apply u_seqNum_reorder_bound with(sent:=encoded)=>//.
-      + rewrite Henc encoder_concat_nochange_eq -encoder_all_steps_concat.
-        apply rse_encode_stream_uniq=>//.
+      + rewrite Henc producer_concat_nochange_eq -producer_all_steps_concat.
+        apply rse_produce_stream_uniq=>//.
         * move=> k' h'. by rewrite /zseq mem_nseq => /andP[_ /eqP[]->->].
         * by rewrite /zseq size_nseq Zlength_size Nat2Z.id.
       + rewrite Henc.
         by apply same_block_index=>//; rewrite -Henc; apply Hsub.
     - move: Hthresh. rewrite !Nat2Z.inj_add. lia.
   }
-  move: Hdec. rewrite (decoder_timeout_notimeout_all Hwf' Hreordup) 
+  move: Hdec. rewrite (consumer_timeout_notimeout_all Hwf' Hreordup) 
     => Hdec.
   (*Now, we use the loss condition to show that enough packets are seen,
     hence we can apply [all_packets_in_block_recovered] to get
@@ -225,7 +225,7 @@ Corollary all_packets_recovered_Z (orig : list packet)
   uniq (map p_seqNum orig) ->
   Zlength enc_params = Zlength orig ->
   all (fun x => x == (k, h)) enc_params ->
-  encoded = (encoder_all_steps orig enc_params).2 ->
+  encoded = (producer_all_steps orig enc_params).2 ->
   (*No new packets are added*)
   (forall p, p \in received -> p \in encoded) ->
   (*At least k packets in i(k+h) to (i+1) (k+h) received, for all i*)
@@ -234,7 +234,7 @@ Corollary all_packets_recovered_Z (orig : list packet)
   (*Bound on reordering and duplication*)
   duplicates_bounded received fpacket_inhab m ->
   reorder_bounded encoded received d ->
-  decoded = (decoder_all_steps threshold received).1.2 ->
+  decoded = (consumer_all_steps threshold received).1.2 ->
   (*Threshold is large enough*)
   (threshold >= k + h + Z.of_nat (2 * d + m))%Z ->
   (*We cannot make guarantees about the last portion of the list*)
@@ -280,7 +280,7 @@ Corollary all_packets_recovered_div_Z (orig : list packet)
   uniq (map p_seqNum orig) ->
   Zlength enc_params = Zlength orig ->
   all (fun x => x == (k, h)) enc_params ->
-  encoded = (encoder_all_steps orig enc_params).2 ->
+  encoded = (producer_all_steps orig enc_params).2 ->
   (*No new packets are added*)
   (forall p, p \in received -> p \in encoded) ->
   (*At least k packets in i(k+h) to (i+1) (k+h) received, for all i*)
@@ -289,7 +289,7 @@ Corollary all_packets_recovered_div_Z (orig : list packet)
   (*Bound on reordering and duplication*)
   duplicates_bounded received fpacket_inhab m ->
   reorder_bounded encoded received d ->
-  decoded = (decoder_all_steps threshold received).1.2 ->
+  decoded = (consumer_all_steps threshold received).1.2 ->
   (*Threshold is large enough*)
   (threshold >= k + h + Z.of_nat (2 * d + m))%Z ->
   (Z.to_nat k) %| size orig ->
@@ -303,7 +303,7 @@ Proof.
   by rewrite divnK // -Zlength_size sublist_same; try lia.
 Qed. 
 
-(*One more collary, combining the two previous ones:
+(*One more corollary, combining the two previous ones:
   under these conditions, the original and decoded streams
   have the same elements up to sequence numbers*)
 Corollary orig_decoded_streams_Z (orig : list packet) 
@@ -315,7 +315,7 @@ Corollary orig_decoded_streams_Z (orig : list packet)
   uniq (map p_seqNum orig) ->
   Zlength enc_params = Zlength orig ->
   all (fun x => x == (k, h)) enc_params ->
-  encoded = (encoder_all_steps orig enc_params).2 ->
+  encoded = (producer_all_steps orig enc_params).2 ->
   (*No new packets are added*)
   (forall p, p \in received -> p \in encoded) ->
   (*At least k packets in i(k+h) to (i+1) (k+h) received for all i*)
@@ -324,7 +324,7 @@ Corollary orig_decoded_streams_Z (orig : list packet)
   (*Bound on reordering and duplication*)
   duplicates_bounded received fpacket_inhab m ->
   reorder_bounded encoded received d ->
-  decoded = (decoder_all_steps threshold received).1.2 ->
+  decoded = (consumer_all_steps threshold received).1.2 ->
   (*Threshold is large enough*)
   (threshold >= k + h + Z.of_nat (2 * d + m))%Z ->
   (Z.to_nat k) %| size orig ->
@@ -356,20 +356,20 @@ Qed.
 End TimeoutCorrect.
 
 (*Now prove these theorems for the machine-length version of the
-  decoder*)
+  Consumer*)
 
 Section Machine.
 
 (*The weakest spec: all data packets that are received by the
-  decoder are returned*)
+  Consumer are returned*)
 Section Weak.
 
-(*Doesn't even need anything about encoder*)
+(*Doesn't even need anything about Producer*)
 Theorem all_data_sent: forall (threshold: int) 
   (received: list fpacket) (p: fpacket),
   p \in received ->
   fd_isParity p = false ->
-  p_packet p \in (decoder_all_steps_m threshold received).1.2.
+  p_packet p \in (consumer_all_steps_m threshold received).1.2.
 Proof.
   apply all_data_outputted_m.
 Qed.
@@ -378,7 +378,7 @@ End Weak.
 
 (*Intermediate spec: if the FEC params are within the correct bounds
   and all packet sequence numbers are at most 2^63-1, then the
-  decoder only outputs packets that were originally given to the encoder,
+  Consumer only outputs packets that were originally given to the Producer,
   modulo sequence numbers.*)
 Section Intermediate.
 
@@ -396,9 +396,9 @@ Theorem all_decoded_in (orig : list packet)
   uniq (map p_seqNum orig) ->
   (forall (p: packet), p \in orig ->
     Z.of_nat (p_seqNum p) < Int64.half_modulus) ->
-  encoded = (encoder_all_steps orig enc_params).2 ->
+  encoded = (producer_all_steps orig enc_params).2 ->
   (forall p, p \in received -> p \in encoded) ->
-  decoded = (decoder_all_steps_m threshold received).1.2 ->
+  decoded = (consumer_all_steps_m threshold received).1.2 ->
   forall p, p \in decoded -> 
     exists p', p' \in orig /\ remove_seqNum p = remove_seqNum p'.
 Proof.
@@ -406,7 +406,7 @@ Proof.
     Hallval Hallenc Huniq Hseqs Henc Hsublist Hdec p Hinp.
   apply (@all_decoded_in_Z upd_time (not_timed_out (Int.unsigned threshold))
     orig encoded received decoded enc_params)=>//.
-  rewrite Hdec decoder_all_steps_m_eq //.
+  rewrite Hdec consumer_all_steps_m_eq //.
   move=> p' Hinp'.
   apply (encoder_bounds Hparams Hallval Hallenc Huniq)=>//.
   - move: Hlenorig. rewrite !Zlength_size. lia.
@@ -442,7 +442,7 @@ Theorem block_i_recovered (orig : list packet)
   Z.of_nat (p_seqNum p) < Int64.half_modulus) ->
   Zlength enc_params = Zlength orig ->
   all (fun x => x == (k, h)) enc_params ->
-  encoded = (encoder_all_steps orig enc_params).2 ->
+  encoded = (producer_all_steps orig enc_params).2 ->
   (*No new packets are added*)
   (forall p, p \in received -> p \in encoded) ->
   (*At least k packets in i(k+h) to (i+1) (k+h) received*)
@@ -451,7 +451,7 @@ Theorem block_i_recovered (orig : list packet)
   (*Bound on reordering and duplication*)
   duplicates_bounded received fpacket_inhab m ->
   reorder_bounded encoded received d ->
-  decoded = (decoder_all_steps_m threshold received).1.2 ->
+  decoded = (consumer_all_steps_m threshold received).1.2 ->
   (*Threshold is large enough but less than 2^30*)
   (k + h + Z.of_nat (2 * d + m) <= Int.unsigned threshold <
     Int.half_modulus / 2)%Z ->
@@ -465,7 +465,7 @@ Proof.
     Hdups Hreord Hdec Hthresh p. 
   apply (@block_i_recovered_Z k h k_bound h_bound orig encoded
     received decoded enc_params d m (Int.unsigned threshold))=>//; try lia.
-  rewrite Hdec decoder_all_steps_m_eq //; try lia.
+  rewrite Hdec consumer_all_steps_m_eq //; try lia.
   move=> p' Hinp'.
   apply (@encoder_bounds orig enc_params)=>//.
   - move=> k' h' Hin.
@@ -485,7 +485,7 @@ Theorem all_packets_recovered (orig : list packet)
     Z.of_nat (p_seqNum p) < Int64.half_modulus) ->
   Zlength enc_params = Zlength orig ->
   all (fun x => x == (k, h)) enc_params ->
-  encoded = (encoder_all_steps orig enc_params).2 ->
+  encoded = (producer_all_steps orig enc_params).2 ->
   (*No new packets are added*)
   (forall p, p \in received -> p \in encoded) ->
   (*At least k packets in i(k+h) to (i+1) (k+h) received for all i*)
@@ -494,7 +494,7 @@ Theorem all_packets_recovered (orig : list packet)
   (*Bound on reordering and duplication*)
   duplicates_bounded received fpacket_inhab m ->
   reorder_bounded encoded received d ->
-  decoded = (decoder_all_steps_m threshold received).1.2 ->
+  decoded = (consumer_all_steps_m threshold received).1.2 ->
   (*Threshold is large enough but less than 2^30*)
   (k + h + Z.of_nat (2 * d + m) <= Int.unsigned threshold <
     Int.half_modulus / 2)%Z ->
@@ -507,7 +507,7 @@ Proof.
     Hdups Hreord Hdec Hthresh p. 
   apply (@all_packets_recovered_Z k h k_bound h_bound orig encoded
     received decoded enc_params d m (Int.unsigned threshold))=>//; try lia.
-  rewrite Hdec decoder_all_steps_m_eq //; try lia.
+  rewrite Hdec consumer_all_steps_m_eq //; try lia.
   move=> p' Hinp'.
   apply (@encoder_bounds orig enc_params)=>//.
   - move=> k' h' Hin.
@@ -529,7 +529,7 @@ Theorem orig_decoded_streams (orig : list packet)
     Z.of_nat (p_seqNum p) < Int64.half_modulus) ->
   Zlength enc_params = Zlength orig ->
   all (fun x => x == (k, h)) enc_params ->
-  encoded = (encoder_all_steps orig enc_params).2 ->
+  encoded = (producer_all_steps orig enc_params).2 ->
  (*No new packets are added*)
  (forall p, p \in received -> p \in encoded) ->
  (*At least k packets in i(k+h) to (i+1) (k+h) received for all i*)
@@ -538,7 +538,7 @@ Theorem orig_decoded_streams (orig : list packet)
   (*Bound on reordering and duplication*)
   duplicates_bounded received fpacket_inhab m ->
   reorder_bounded encoded received d ->
-  decoded = (decoder_all_steps_m threshold received).1.2 ->
+  decoded = (consumer_all_steps_m threshold received).1.2 ->
   (*Threshold is large enough but less than 2^30*)
   (k + h + Z.of_nat (2 * d + m) <= Int.unsigned threshold <
     Int.half_modulus / 2)%Z ->
@@ -549,7 +549,7 @@ Proof.
     Hdups Hreord Hdec Hthresh p. 
   apply (@orig_decoded_streams_Z k h k_bound h_bound orig encoded
     received decoded enc_params d m (Int.unsigned threshold))=>//; try lia.
-  rewrite Hdec decoder_all_steps_m_eq //; try lia.
+  rewrite Hdec consumer_all_steps_m_eq //; try lia.
   move=> p' Hinp'.
   apply (@encoder_bounds orig enc_params)=>//.
   - move=> k' h' Hin.
